theories/tree_borrows/wishlist.v
@@ -77,6 +77,42 @@ Lemma trees_equal_allows_same_access C tr1 tr2 blk ev1 ev2 ev3 ev4 kind acc_tg r
   is_Some (apply_within_trees (memory_access kind C acc_tg range) blk tr2).
 Admitted.
 
+Lemma wf_tree_tree_unique tr ev1 ev2 :
+  wf_tree tr ev1 ev2 →
+  ∀ tg,
+  tree_contains tg tr →
+  tree_unique tg tr.
+Proof.
+  intros Hwf tg Hcont.
+  by destruct (Hwf tg Hcont) as (? & H & _).
+Qed.
+
+Lemma trees_equal_preserved_by_access
+  {C blk tr1 tr2 tr1' tr2' kind acc_tg range ev1 ev2 ev3 ev4}
+  :
+  wf_trees tr1 ev1 ev2 →
+  wf_trees tr2 ev3 ev4 →
+  trees_equal C tr1 tr2 ->
+  trees_contain acc_tg tr1 blk ->
+  apply_within_trees (memory_access kind C acc_tg range) blk tr1 = Some tr1' ->
+  apply_within_trees (memory_access kind C acc_tg range) blk tr2 = Some tr2' ->
+  trees_equal C tr1' tr2'.
+Proof.
+  intros Hwf1 Hwf2 Heq Hcont.
+  intros ((tr1blk & tr1blk' & Hlutr1 & Hlutr1' & Hacc1) & Htr1nblk)%apply_within_trees_lookup.
+  intros ((tr2blk & tr2blk' & Hlutr2 & Hlutr2' & Hacc2) & Htr2nblk)%apply_within_trees_lookup.
+  intros blk'. destruct (decide (blk = blk')) as [<- | Hne];
+    last rewrite -Htr1nblk // -Htr2nblk //.
+  rewrite Hlutr1' Hlutr2'. econstructor.
+  specialize (Heq blk).
+  rewrite Hlutr1 Hlutr2 in Heq.
+  inversion Heq as [x1 x2 Heq1|]; subst x1 x2. (* yikes *)
+  eapply tree_equal_preserved_by_access.
+  3, 5, 6: done.
+  3: rewrite /trees_contain /trees_at_block Hlutr1 // in Hcont.
+  all: eapply wf_tree_tree_unique; (match goal with [ H : wf_trees _ _ _ |- _] => by eapply H end).
+Qed.
+
 Lemma apply_trees_access_lookup_general offi cids ev1 ev2 trs kind blk off1 sz acc_tg lu_tg trs' itold :
   apply_within_trees (memory_access kind cids acc_tg (off1, sz)) blk trs = Some trs' →
   wf_trees trs ev1 ev2 →
@@ -128,6 +164,50 @@ Proof.
     rewrite /item_lookup /= permSome //=.
 Qed.
 
+Lemma apply_trees_access_lookup_outside blki offi cids ev1 ev2 trs kind blk off1 sz acc_tg lu_tg trs' itold :
+  apply_within_trees (memory_access kind cids acc_tg (off1, sz)) blk trs = Some trs' →
+  wf_trees trs ev1 ev2 →
+  ¬ (blki = blk ∧ off1 ≤ offi < off1 + sz) →
+  trees_lookup trs blki lu_tg itold →
+  ∃       itnew, trees_lookup trs' blki lu_tg itnew ∧
+                 let permold := item_lookup itold offi in let permnew := item_lookup itnew offi in
+                 initp itold = initp itnew ∧
+                 iprot itold = iprot itnew ∧
+                 permold = permnew.
+Proof.
+  intros App wf OutOfBounds Lookup.
+  rewrite /apply_within_trees in App.
+  rewrite bind_Some in App.
+  destruct App as [tr [trSome Acc]].
+  rewrite bind_Some in Acc.
+  destruct Acc as [tr' [Acc Out]].
+  injection Out; intros; subst; clear Out.
+  destruct (decide (blk = blki)) as [->|Hne]; last first.
+  { destruct Lookup as (it & Hit1 & Hit2). exists itold. split_and!; try done.
+    exists it; split; last done.
+    by rewrite lookup_insert_ne. }
+  assert (tree_contains lu_tg tr) as Ex. {
+    eapply trees_at_block_projection; [|eassumption].
+    eapply trees_contain_trees_lookup_2.
+    eassumption.
+  }
+  assert (tree_item_determined lu_tg itold tr) as Det. {
+    destruct Lookup as [trbis [trsLookup trLookup]].
+    assert (trbis = tr) by congruence. subst.
+    apply trLookup.
+  }
+  destruct (apply_access_spec_per_node Ex Det Acc) as [itnew [itAcc [Ex' Det']]].
+  rewrite /item_apply_access in itAcc. symmetry in itAcc.
+  apply bind_Some in itAcc as (permsnew&Hpermsnew&[= Hitnew]).
+  exists itnew. split.
+  { exists tr'. split; first by rewrite lookup_insert. done. }
+  subst itnew. simpl. split_and!; try done.
+  rewrite /item_lookup; simpl. f_equal.
+  eapply (mem_apply_range'_spec _ _ offi) in Hpermsnew.
+  destruct (decide (range'_contains _ _)) as [Hinrange|_]; last done.
+  exfalso. eapply OutOfBounds. split; first done. apply Hinrange.
+Qed.
+
 
 Lemma apply_trees_access_lookup_same_tag cids ev1 ev2 trs kind blk off1 sz offi tg trs':
   apply_within_trees (memory_access kind cids tg (off1, sz)) blk trs = Some trs' →
@@ -148,5 +228,54 @@ Proof.
   split; first assumption.
   apply newSpec.
 Qed.
+
+
+(* TODO move somewhere else *)
+Lemma tag_protected_preserved_by_access tg_acc tg_prs l C c trs trs' acc blk off sz ev1 ev2 :
+  wf_trees trs ev1 ev2 →
+  apply_within_trees (memory_access acc C tg_acc (off, sz)) blk trs = Some trs' →
+  call_is_active c C →
+  tag_protected_for c trs  l tg_prs →
+  tag_protected_for c trs' l tg_prs.
+Proof.
+  intros Hwf Hwithin Hcall (it & Hlu & Hprot & Hinit). 
+  destruct (decide (l.1 = blk ∧ (off ≤ l.2 < off + sz))%Z) as [(<- & Hin)|Hout].
+  - eapply apply_trees_access_lookup_general in Hlu as (itnew & Hlunew & Heqinit & Heqprot & Hacc); [|done..].
+    exists itnew. split; first done.
+    split; first by rewrite -Heqprot.
+    intros Hperminit.
+    assert (protector_is_active (iprot itnew) C) as Hactive.
+    { exists c. rewrite -Heqprot. done. }
+    apply bind_Some in Hacc as (perm1 & Hacc & (perm2 & Htrigger & [= Heqperm])%bind_Some).
+    rewrite -Heqperm /= in Hperminit |- *.
+    rewrite (bool_decide_eq_true_2 _ Hactive) /= in Hacc, Htrigger.
+    rewrite /apply_access_perm_inner in Hacc.
+    destruct (initialized (item_lookup it l.2));
+      [ specialize (Hinit eq_refl) | injection Htrigger as -> ].
+    all: destruct trees_rel_dec eqn:Hreldec; destruct acc; destruct (perm (item_lookup it l.2)) as [[] []| | |] eqn:Hpermold; simplify_eq; try done;
+         repeat (simplify_eq; try done; destruct bool_decide; (try simpl in Htrigger); simplify_eq; try done).
+  - eapply apply_trees_access_lookup_outside in Hlu as (itnew & Hlunew & Heqinit & Heqprot & Hacc); [|done..].
+    exists itnew. split; first done.
+    split; first by rewrite -Heqprot.
+    by rewrite -Hacc.
+Qed.
+
+
+
+
+
+
+
+
+
+
+
+
+
+
+
+
+
+
 
 
